checker/theories/Substitution.v
@@ -215,7 +215,7 @@ Proof.
   generalize #|mfix| at 2 3. induction n0; auto. simpl.
   f_equal. apply IHn0.
 Qed.
-Hint Resolve subst_unfold_fix.
+Hint Resolve subst_unfold_fix : core.
 
 Lemma subst_unfold_cofix n k mfix idx narg fn :
   All Ast.wf n ->
@@ -231,7 +231,7 @@ Proof.
   generalize #|mfix| at 2 3. induction n0; auto. simpl.
   f_equal. apply IHn0.
 Qed.
-Hint Resolve subst_unfold_cofix.
+Hint Resolve subst_unfold_cofix : core.
 
 Lemma subst_is_constructor:
   forall (args : list term) (narg : nat) n k,
@@ -244,8 +244,8 @@ Proof.
   destruct t; try discriminate || reflexivity. simpl.
   destruct args0; auto.
 Qed.
-Hint Resolve subst_is_constructor.
-Hint Constructors All_local_env.
+Hint Resolve subst_is_constructor : core.
+Hint Constructors All_local_env : core.
 
 Lemma typed_subst `{checker_flags} Σ Γ t T n k :
   wf Σ.1 -> k >= #|Γ| ->
