pcuic/theories/PCUICGeneration.v
@@ -1,4 +1,5 @@
 (* Distributed under the terms of the MIT license.   *)
+Require Import Equations.Prop.DepElim.
 From Equations Require Import Equations.
 From Coq Require Import Bool String List Program BinPos Compare_dec.
 From MetaCoq.Template Require Import config utils.
@@ -10,7 +11,6 @@ Require Import String.
 From MetaCoq Require Import LibHypsNaming.
 Local Open Scope string_scope.
 Set Asymmetric Patterns.
-Require Import Equations.Prop.DepElim.
 
 Section Generation.
   Context `{cf : config.checker_flags}.
@@ -61,13 +61,13 @@ Section Generation.
     - assumption.
     - simpl. cbn. eapply ih.
       simpl in h. pose proof (typing_wf_local h) as hc.
-      dependent induction hc. all: inversion H. subst.
-      cbn in t1, t0. destruct t0.
+      dependent induction hc. 
+      cbn in t1, t2. destruct t1.
       econstructor ; eassumption.
     - simpl. cbn. eapply ih.
       pose proof (typing_wf_local h) as hc. cbn in hc.
-      dependent induction hc. all: inversion H. subst.
-      cbn in t0. destruct t0.
+      dependent induction hc.
+      cbn in t1. destruct t1.
       econstructor ; eassumption.
   Qed.
 
