pcuic/theories/PCUICValidity.v
@@ -6,8 +6,8 @@ From MetaCoq.PCUIC Require Import PCUICAst PCUICAstUtils PCUICInduction
      PCUICParallelReductionConfluence PCUICConfluence PCUICUnivSubst
      PCUICUnivSubstitution PCUICConversion PCUICPrincipality.
 
-From Equations Require Import Equations.
 Require Import Equations.Prop.DepElim.
+From Equations Require Import Equations.
 Require Import ssreflect.
 
 Derive NoConfusion for term.
