pcuic/theories/TemplateToPCUICCorrectness.v
@@ -8,8 +8,8 @@ From MetaCoq.Template Require Import config utils AstUtils BasicAst Ast
 From MetaCoq.PCUIC Require Import PCUICAst PCUICAstUtils PCUICInduction
      PCUICLiftSubst PCUICEquality
      PCUICUnivSubst PCUICTyping PCUICGeneration TemplateToPCUIC.
-From Equations Require Import Equations.
 Require Import Equations.Prop.DepElim.
+From Equations Require Import Equations.
 
 Require Import String.
 Local Open Scope string_scope.
